theories/ordinals/Ackermann/LNN2LNT.v
@@ -41,29 +41,29 @@ Proof.
   - simpl; now rewrite Hrecn.
 Qed.
 
-Lemma LNN2LNT_freeVarTerm (t : fol.Term LNN):
- freeVarTerm LNT (LNN2LNT_term t) = freeVarTerm LNN t.
+Lemma LNN2LNT_freeVarT (t : fol.Term LNN):
+ freeVarT LNT (LNN2LNT_term t) = freeVarT LNN t.
 Proof.
   induction t using
     Term_Terms_ind
     with
     (P0 := fun (n : nat) (ts : fol.Terms LNN n) =>
-             freeVarTerms LNT n (LNN2LNT_terms n ts) = freeVarTerms LNN n ts).
+             freeVarTs LNT n (LNN2LNT_terms n ts) = freeVarTs LNN n ts).
   - intros; reflexivity.
-  - intros; simpl; repeat rewrite freeVarTermApply; now apply IHt.
+  - intros; simpl; repeat rewrite freeVarTApply; now apply IHt.
   - intros; simpl; reflexivity. 
-  - transitivity (freeVarTerm LNN t ++ freeVarTerms LNN n t0).
+  - transitivity (freeVarT LNN t ++ freeVarTs LNN n t0).
     + rewrite <- IHt0; rewrite <- IHt; reflexivity.
     + reflexivity.
 Qed.
 
-Lemma LNN2LNT_freeVarTerms (n : nat) (ts : fol.Terms LNN n):
-    freeVarTerms LNT n (LNN2LNT_terms n ts) = freeVarTerms LNN n ts.
+Lemma LNN2LNT_freeVarTs (n : nat) (ts : fol.Terms LNN n):
+    freeVarTs LNT n (LNN2LNT_terms n ts) = freeVarTs LNN n ts.
 Proof.
   induction ts as [| n t ts Hrects].
   - reflexivity.
-  - simpl; transitivity (freeVarTerm LNN t ++ freeVarTerms LNN n ts).
-    + rewrite <- Hrects; rewrite <- LNN2LNT_freeVarTerm; reflexivity.
+  - simpl; transitivity (freeVarT LNN t ++ freeVarTs LNN n ts).
+    + rewrite <- Hrects; rewrite <- LNN2LNT_freeVarT; reflexivity.
     + reflexivity.
 Qed.
 
@@ -225,7 +225,7 @@ Lemma LNN2LNT_freeVarF (f : fol.Formula LNN) (v : nat):
     In v (freeVarF LNN f).
 Proof.
   induction f as [t t0| r t| f1 Hrecf1 f0 Hrecf0| f Hrecf| n f Hrecf].
-  - simpl; repeat rewrite LNN2LNT_freeVarTerm; tauto.
+  - simpl; repeat rewrite LNN2LNT_freeVarT; tauto.
   - destruct r. (* is LT *)
     simpl. 
     destruct (consTerms _ _ t) as [(a,b) p].
@@ -234,19 +234,19 @@ Proof.
     simpl in p0; rewrite <- p0.
     rewrite translateLT1.
     rewrite <- (nilTerms _ b0).
-    unfold freeVarTerms in |- *.
-    fold (freeVarTerm LNN) in |- *.
+    unfold freeVarTs in |- *.
+    fold (freeVarT LNN) in |- *.
     rewrite <- app_nil_end.
     split.
     + intros H; decompose record (freeVarSubAllFormula1 _ _ _ _ H) /r.
       intros H x [H0| H0] H2.
       * rewrite <- H0 in H2.
         simpl in H2.
-        rewrite LNN2LNT_freeVarTerm in H2; auto with datatypes.
+        rewrite LNN2LNT_freeVarT in H2; auto with datatypes.
       * destruct H0 as [H0| H0].
         -- rewrite <- H0 in H2.
            simpl in H2.
-           rewrite LNN2LNT_freeVarTerm in H2.
+           rewrite LNN2LNT_freeVarT in H2.
            auto with datatypes.
         -- contradiction.
     + intro H; destruct (in_app_or _ _ _ H) as [H0 | H0].
@@ -255,7 +255,7 @@ Proof.
         left.
         reflexivity.
         simpl in |- *.
-        rewrite LNN2LNT_freeVarTerm.
+        rewrite LNN2LNT_freeVarT.
         auto.
       * eapply freeVarSubAllFormula2.
         simpl in |- *.
@@ -263,7 +263,7 @@ Proof.
         left.
         reflexivity.
         simpl in |- *.
-        rewrite LNN2LNT_freeVarTerm.
+        rewrite LNN2LNT_freeVarT.
         auto.
   - simpl in |- *.
     induction Hrecf1 as (H, H0).
@@ -414,7 +414,7 @@ Proof.
         -- auto.
         -- contradiction.
         -- elim H4.
-        rewrite LNN2LNT_freeVarTerm.
+        rewrite LNN2LNT_freeVarT.
         assumption.
         -- apply (reduceForall LNT).
            apply (notInFreeVarSys LNT).
@@ -445,7 +445,7 @@ Proof.
            eapply iffTrans.
            apply (subFormulaExch LNT).
            auto.
-           rewrite LNN2LNT_freeVarTerm.
+           rewrite LNN2LNT_freeVarT.
            auto.
            simpl in |- *.
            tauto.
@@ -505,25 +505,25 @@ Proof.
   - intros n t0 H t1 H0; now rewrite H, H0.
 Qed.
 
-Lemma LNT2LNN_freeVarTerm ( t : Term):
-  freeVarTerm LNN (LNT2LNN_term t) = freeVarTerm LNT t.
+Lemma LNT2LNN_freeVarT ( t : Term):
+  freeVarT LNN (LNT2LNN_term t) = freeVarT LNT t.
 Proof.
   elim t using
     Term_Terms_ind
     with
     (P0 := fun (n : nat) (ts : fol.Terms LNT n) =>
-             freeVarTerms _ n (LNT2LNN_terms n ts) = freeVarTerms LNT n ts);
+             freeVarTs _ n (LNT2LNN_terms n ts) = freeVarTs LNT n ts);
     simpl in |- *.  
   - reflexivity.
   - intros f t0 H; transitivity
-                     (freeVarTerms LNN (LNTFunctionArity f)
+                     (freeVarTs LNN (LNTFunctionArity f)
                         (LNT2LNN_terms (LNTFunctionArity f) t0)).
     + reflexivity.
     + now rewrite H.
   - reflexivity.
   - intros n t0 H t1 H0; transitivity
-                           (freeVarTerm LNN (LNT2LNN_term t0) ++
-                              freeVarTerms LNN n (LNT2LNN_terms n t1)).
+                           (freeVarT LNN (LNT2LNN_term t0) ++
+                              freeVarTs LNN n (LNT2LNN_terms n t1)).
     + reflexivity.
     + now rewrite H, H0.
 Qed.
@@ -533,7 +533,7 @@ Lemma LNT2LNN_freeVarF (f : Formula):
 Proof.
   induction f as [t t0| r t| f1 Hrecf1 f0 Hrecf0| f Hrecf| n f Hrecf];
     simpl in |- *.
-  - repeat rewrite LNT2LNN_freeVarTerm; reflexivity.
+  - repeat rewrite LNT2LNN_freeVarT; reflexivity.
   - destruct r.
   - now rewrite Hrecf1,  Hrecf0.
   - assumption.
@@ -557,8 +557,8 @@ Proof.
       rewrite (subFormulaForall LNT), (subFormulaForall LNN).
     destruct (eq_nat_dec v v0) as [e | n].
     + reflexivity.
-    + rewrite LNT2LNN_freeVarTerm.
-      destruct (In_dec eq_nat_dec v (freeVarTerm LNT s)) as [i | i].
+    + rewrite LNT2LNN_freeVarT.
+      destruct (In_dec eq_nat_dec v (freeVarT LNT s)) as [i | i].
       * simpl; repeat rewrite H; simpl. 
         -- now rewrite LNT2LNN_freeVarF.
         -- apply depthForall.
