theories/ordinals/Ackermann/subProp.v
@@ -26,16 +26,16 @@ Let SysPrf := SysPrf L.
 
 Lemma freeVarSubTerm1 (t : Term):
   forall  (v : nat) (s : Term) (x : nat),
-    In x (freeVarTerm L t) ->
-    v <> x -> In x (freeVarTerm L (substT L t v s)).
+    In x (freeVarT L t) ->
+    v <> x -> In x (freeVarT L (substT L t v s)).
 Proof.
   elim t using
     Term_Terms_ind
     with
     (P0 := fun (n : nat) (ts : fol.Terms L n) =>
              forall (v : nat) (s : Term) (x : nat),
-               In x (freeVarTerms L n ts) ->
-               v <> x -> In x (freeVarTerms L n (substTs L n ts v s))).
+               In x (freeVarTs L n ts) ->
+               v <> x -> In x (freeVarTs L n (substTs L n ts v s))).
   -  intros n v s x H H0; simpl.
      induction (eq_nat_dec v n) as [? | ?].
      + destruct H0; simpl in H; induction H as [H| H].
@@ -43,24 +43,24 @@ Proof.
        * contradiction.
      + assumption.
   - intros f t0 H v s x H0 H1; simpl in |- *.
-    unfold freeVarTerm; apply H; auto.
+    unfold freeVarT; apply H; auto.
   - intros; auto.
-  - intros n t0 H t1 H0 v s x H1 H2; unfold freeVarTerms in H1.
+  - intros n t0 H t1 H0 v s x H1 H2; unfold freeVarTs in H1.
     induction (in_app_or _ _ _ H1);
-      unfold freeVarTerms; simpl; apply in_or_app; auto.
+      unfold freeVarTs; simpl; apply in_or_app; auto.
 Qed.
 
 Lemma freeVarSubTerms1 (n : nat) (ts : Terms n) (v : nat) (s : Term) (x : nat):
-  In x (freeVarTerms L n ts) ->
-  v <> x -> In x (freeVarTerms L n (substTs L n ts v s)).
+  In x (freeVarTs L n ts) ->
+  v <> x -> In x (freeVarTs L n (substTs L n ts v s)).
 Proof.
   intros H H0; induction ts as [| n t ts Hrects].
   - auto.
-  - unfold freeVarTerms in H; fold (freeVarTerm L t) in H.
-    fold (freeVarTerms L _ ts) in H.
-    unfold freeVarTerms; simpl;
-      fold (freeVarTerm L (substT L t v s));
-      fold (freeVarTerms L n (substTs L n ts v s));
+  - unfold freeVarTs in H; fold (freeVarT L t) in H.
+    fold (freeVarTs L _ ts) in H.
+    unfold freeVarTs; simpl;
+      fold (freeVarT L (substT L t v s));
+      fold (freeVarTs L n (substTs L n ts v s));
       apply in_or_app.
     induction (in_app_or _ _ _ H).
     + left; apply freeVarSubTerm1; auto.
@@ -87,10 +87,10 @@ Proof.
     - intros v a H v0 s x H0 H1; rewrite subFormulaForall; 
         induction (eq_nat_dec v v0) as [? | b].
       + auto.
-      + induction (In_dec eq_nat_dec v (freeVarTerm L s)) as [a0 | ?].
-        * set (nv := newVar (v0 :: freeVarTerm L s ++ freeVarF L a)).
+      + induction (In_dec eq_nat_dec v (freeVarT L s)) as [a0 | ?].
+        * set (nv := newVar (v0 :: freeVarT L s ++ freeVarF L a)).
           simpl; apply in_in_remove.
-          --  intro H2; elim (newVar1 (v0 :: freeVarTerm L s ++ freeVarF L a)).
+          --  intro H2; elim (newVar1 (v0 :: freeVarT L s ++ freeVarF L a)).
               fold nv; simpl; right; apply in_or_app; right; eapply in_remove.
               rewrite <- H2; apply H1.
           -- apply H.
@@ -111,30 +111,30 @@ Qed.
 
 Lemma freeVarSubTerm2 (t : Term) :
   forall  (v : nat) (s : Term) (x : nat),
-    In x (freeVarTerm L s) ->
-    In v (freeVarTerm L t) -> In x (freeVarTerm L (substT L t v s)).
+    In x (freeVarT L s) ->
+    In v (freeVarT L t) -> In x (freeVarT L (substT L t v s)).
 Proof.
   elim t using Term_Terms_ind 
     with
     (P0 := fun (n : nat) (ts : fol.Terms L n) =>
              forall (v : nat) (s : Term) (x : nat),
-               In x (freeVarTerm L s) ->
-               In v (freeVarTerms L n ts) ->
-               In x (freeVarTerms L n (substTs L n ts v s))).
+               In x (freeVarT L s) ->
+               In v (freeVarTs L n ts) ->
+               In x (freeVarTs L n (substTs L n ts v s))).
   - intros n v s x H H0; simpl; induction (eq_nat_dec v n) as [? | b].
     + assumption.
     +  elim b; induction H0 as [H0| H0].
           * auto.
           * contradiction.
-  - intros f t0 H v s x H0 H1; simpl; unfold freeVarTerm;
+  - intros f t0 H v s x H0 H1; simpl; unfold freeVarT;
       fold
-        (freeVarTerms L _ (substTs L (arityF L f) t0 v s)).
+        (freeVarTs L _ (substTs L (arityF L f) t0 v s)).
     apply H; auto.
   - intros v s x H H0; auto.
-  - intros n t0 H t1 H0 v s x H1 H2; simpl; unfold freeVarTerms in H2;
-    fold (freeVarTerm L t0) in H2; fold (freeVarTerms L n t1) in H2.
-    unfold freeVarTerms; fold (freeVarTerm L (substT L t0 v s));
-      fold (freeVarTerms L n (substTs L n t1 v s));
+  - intros n t0 H t1 H0 v s x H1 H2; simpl; unfold freeVarTs in H2;
+    fold (freeVarT L t0) in H2; fold (freeVarTs L n t1) in H2.
+    unfold freeVarTs; fold (freeVarT L (substT L t0 v s));
+      fold (freeVarTs L n (substTs L n t1 v s));
       apply in_or_app.
     induction (in_app_or _ _ _ H2).
     + left; apply H; auto.
@@ -142,16 +142,16 @@ Proof.
 Qed.
 
 Lemma freeVarSubTerms2 (n : nat) (ts : Terms n) (v : nat) (s : Term) (x : nat):
- In x (freeVarTerm L s) ->
- In v (freeVarTerms L n ts) ->
- In x (freeVarTerms L n (substTs L n ts v s)).
+ In x (freeVarT L s) ->
+ In v (freeVarTs L n ts) ->
+ In x (freeVarTs L n (substTs L n ts v s)).
 Proof.
   intros H H0; induction ts as [| n t ts Hrects].
   - contradiction H0. 
-  - simpl; unfold freeVarTerms in H0; fold (freeVarTerm L t) in H0.
-    fold (freeVarTerms L n ts) in H0; unfold freeVarTerms.
-    fold (freeVarTerm L (substT L t v s));
-      fold (freeVarTerms L n (substTs L n ts v s));
+  - simpl; unfold freeVarTs in H0; fold (freeVarT L t) in H0.
+    fold (freeVarTs L n ts) in H0; unfold freeVarTs.
+    fold (freeVarT L (substT L t v s));
+      fold (freeVarTs L n (substTs L n ts v s));
       apply in_or_app.
     destruct (in_app_or _ _ _ H0).
     + left; apply freeVarSubTerm2; auto.
@@ -160,7 +160,7 @@ Qed.
 
 Lemma freeVarSubFormula2 (f : Formula):
   forall  (v : nat) (s : Term) (x : nat),
-    In x (freeVarTerm L s) ->
+    In x (freeVarT L s) ->
     In v (freeVarF L f) ->
     In x (freeVarF L (substF L f v s)).
 Proof.
@@ -181,11 +181,11 @@ Proof.
   - intros v a H v0 s x H0 H1; rewrite subFormulaForall.
     induction (eq_nat_dec v v0).
     + simpl in H1; elim (in_remove_neq _ eq_nat_dec _ _ _ H1); auto. 
-    + induction (In_dec eq_nat_dec v (freeVarTerm L s)) as [a0 | b0].
-      * set (nv := newVar (v0 :: freeVarTerm L s ++ freeVarF L a)).
+    + induction (In_dec eq_nat_dec v (freeVarT L s)) as [a0 | b0].
+      * set (nv := newVar (v0 :: freeVarT L s ++ freeVarF L a)).
         simpl; apply in_in_remove.
         -- intro H2; 
-             elim (newVar1 (v0 :: freeVarTerm L s ++ freeVarF L a)).
+             elim (newVar1 (v0 :: freeVarT L s ++ freeVarF L a)).
            fold nv; simpl; right.
            apply in_or_app.
            rewrite <- H2; auto.
@@ -209,18 +209,18 @@ Qed.
 
 Lemma freeVarSubTerm3  (t : Term):
   forall (v : nat) (s : Term) (x : nat),
-    In x (freeVarTerm L (substT L t v s)) ->
-    In x (List.remove eq_nat_dec v (freeVarTerm L t)) \/
-      In x (freeVarTerm L s).
+    In x (freeVarT L (substT L t v s)) ->
+    In x (List.remove eq_nat_dec v (freeVarT L t)) \/
+      In x (freeVarT L s).
 Proof.
   elim t using
     Term_Terms_ind
     with
     (P0 := fun (n : nat) (ts : fol.Terms L n) =>
              forall (v : nat) (s : Term) (x : nat),
-               In x (freeVarTerms L n (substTs L n ts v s)) ->
-               In x (List.remove eq_nat_dec v (freeVarTerms L n ts)) \/
-                 In x (freeVarTerm L s)). 
+               In x (freeVarTs L n (substTs L n ts v s)) ->
+               In x (List.remove eq_nat_dec v (freeVarTs L n ts)) \/
+                 In x (freeVarT L s)). 
   - intros n v s x H; simpl in H.
     induction (eq_nat_dec v n) as [a | b].
     + now right.
@@ -232,50 +232,50 @@ Proof.
   - intros f t0 H v s x H0; simpl in H0; induction (H _ _ _ H0); auto.
   - auto.
   - intros n t0 H t1 H0 v s x H1; simpl in H1;
-      unfold freeVarTerms in H1;
-      fold (freeVarTerm L (substT L t0 v s)) in H1;
-      fold (freeVarTerms L n (substTs L n t1 v s)) in H1.
+      unfold freeVarTs in H1;
+      fold (freeVarT L (substT L t0 v s)) in H1;
+      fold (freeVarTs L n (substTs L n t1 v s)) in H1.
     destruct (in_app_or _ _ _ H1) as [H2 | H2].
     + induction (H _ _ _ H2) as [H3 | H3].
       * left; apply in_in_remove.
         --  eapply in_remove_neq; apply H3.
-        -- unfold freeVarTerms; apply in_or_app; left.
+        -- unfold freeVarTs; apply in_or_app; left.
            eapply in_remove; apply H3.
       *  auto.
     + induction (H0 _ _ _ H2) as [H3 | H3].
       * left; apply in_in_remove.
         -- eapply in_remove_neq; apply H3.
-        -- unfold freeVarTerms; fold (freeVarTerm L t0);
-             fold (freeVarTerms L n t1); apply in_or_app.
+        -- unfold freeVarTs; fold (freeVarT L t0);
+             fold (freeVarTs L n t1); apply in_or_app.
            right; eapply in_remove; apply H3.
       * auto.
 Qed.
 
 Lemma freeVarSubTerms3 (n : nat) (ts : fol.Terms L n) (v : nat) 
   (s : Term) (x : nat):
-  In x (freeVarTerms L n (substTs L n ts v s)) ->
-  In x (List.remove  eq_nat_dec v (freeVarTerms L n ts)) \/
-    In x (freeVarTerm L s).
+  In x (freeVarTs L n (substTs L n ts v s)) ->
+  In x (List.remove  eq_nat_dec v (freeVarTs L n ts)) \/
+    In x (freeVarT L s).
 Proof.
   intros H; induction ts as [| n t ts Hrects].
   - left; apply H. 
-  - simpl in H; unfold freeVarTerms in H;
-      fold (freeVarTerm L (substT L t v s)) in H;
-      fold (freeVarTerms L n (substTs L n ts v s)) in H;
+  - simpl in H; unfold freeVarTs in H;
+      fold (freeVarT L (substT L t v s)) in H;
+      fold (freeVarTs L n (substTs L n ts v s)) in H;
       induction (in_app_or _ _ _ H) as [H0 | H0].
     + induction (freeVarSubTerm3 _ _ _ _ H0) as [H1 | H1].
       * left.
         apply in_in_remove.
         -- eapply in_remove_neq; apply H1.
-        -- unfold freeVarTerms; fold (freeVarTerm L t);
-             fold (freeVarTerms L n ts); apply in_or_app.
+        -- unfold freeVarTs; fold (freeVarT L t);
+             fold (freeVarTs L n ts); apply in_or_app.
            left; eapply in_remove; apply H1.
       * now right.
     + induction (Hrects H0) as [H1 | H1].
       * left; apply in_in_remove.
         -- eapply in_remove_neq; apply H1.
-        -- unfold freeVarTerms; fold (freeVarTerm L t);
-             fold (freeVarTerms L n ts); apply in_or_app; right.
+        -- unfold freeVarTs; fold (freeVarT L t);
+             fold (freeVarTs L n ts); apply in_or_app; right.
            eapply in_remove; apply H1.
       * now right.
 Qed.
@@ -284,7 +284,7 @@ Lemma freeVarSubFormula3  (f : Formula):
  forall (v : nat) (s : Term) (x : nat),
  In x (freeVarF L (substF L f v s)) ->
  In x (List.remove  eq_nat_dec v (freeVarF L f)) \/
- In x (freeVarTerm L s).
+ In x (freeVarT L s).
 Proof.
   elim f using Formula_depth_ind2. 
   - intros t t0 v s x H; rewrite subFormulaEqual in H.
@@ -321,8 +321,8 @@ Proof.
     + left; apply in_in_remove.
       * eapply in_remove_neq; rewrite <- a0; apply H0.
       * apply H0.
-    + induction (In_dec eq_nat_dec v (freeVarTerm L s)) as [a0 | ?].
-      * set (nv := newVar (v0 :: freeVarTerm L s ++ freeVarF L a)).
+    + induction (In_dec eq_nat_dec v (freeVarT L s)) as [a0 | ?].
+      * set (nv := newVar (v0 :: freeVarT L s ++ freeVarF L a)).
         induction (eq_nat_dec x v) as [a1 | ?].
         -- rewrite a1;  now right.
         -- assert
@@ -373,17 +373,17 @@ Qed.
 
 Lemma freeVarSubTerm4 (t : Term) :
  forall  (v : nat) (s : Term) (x : nat),
- In x (freeVarTerm L (substT L t v s)) ->
- ~ In v (freeVarTerm L t) -> In x (freeVarTerm L t).
+ In x (freeVarT L (substT L t v s)) ->
+ ~ In v (freeVarT L t) -> In x (freeVarT L t).
 Proof.
   elim t using
     Term_Terms_ind
     with
     (P0 := fun (n : nat) (ts : fol.Terms L n) =>
              forall (v : nat) (s : Term) (x : nat),
-               In x (freeVarTerms L n (substTs L n ts v s)) ->
-               ~ In v (freeVarTerms L n ts) -> 
-               In x (freeVarTerms L n ts)).
+               In x (freeVarTs L n (substTs L n ts v s)) ->
+               ~ In v (freeVarTs L n ts) -> 
+               In x (freeVarTs L n ts)).
   - intros n v s x H H0; simpl in H |- *.
     induction (eq_nat_dec v n) as [a | ?].
     + elim H0; rewrite a; simpl; now left. 
@@ -393,46 +393,46 @@ Proof.
     + apply H1.
   - intros; assumption.
   - intros n t0 H t1 H0 v s x H1 H2; simpl in H1.
-    unfold freeVarTerms in H1;
-    fold (freeVarTerm L (substT L t0 v s)) in H1;
-    fold (freeVarTerms L n (substTs L n t1 v s)) in H1;
-    unfold freeVarTerms ;
-      fold (freeVarTerm L t0); fold (freeVarTerms L n t1).
+    unfold freeVarTs in H1;
+    fold (freeVarT L (substT L t0 v s)) in H1;
+    fold (freeVarTs L n (substTs L n t1 v s)) in H1;
+    unfold freeVarTs ;
+      fold (freeVarT L t0); fold (freeVarTs L n t1).
     induction (in_app_or _ _ _ H1) as [H3 | H3].
     + apply in_or_app; left; eapply H.
       * apply H3.
       * intro H4; elim H2.
-        unfold freeVarTerms; fold (freeVarTerm L t0);
-          fold (freeVarTerms L n t1); apply in_or_app.
+        unfold freeVarTs; fold (freeVarT L t0);
+          fold (freeVarTs L n t1); apply in_or_app.
         now left. 
     + apply in_or_app; right; eapply H0.
       * apply H3.
       *  intro H4; elim H2.
-         unfold freeVarTerms; fold (freeVarTerm L t0); 
-           fold (freeVarTerms L n t1); apply in_or_app; now right.
+         unfold freeVarTs; fold (freeVarT L t0); 
+           fold (freeVarTs L n t1); apply in_or_app; now right.
 Qed.
 
 Lemma freeVarSubTerms4 (n : nat) (ts : Terms n) (v : nat)
   (s : Term) (x : nat):
-  In x (freeVarTerms L n (substTs L n ts v s)) ->
-  ~ In v (freeVarTerms L n ts) -> In x (freeVarTerms L n ts).
+  In x (freeVarTs L n (substTs L n ts v s)) ->
+  ~ In v (freeVarTs L n ts) -> In x (freeVarTs L n ts).
 Proof.
   intros H H0; induction ts as [| n t ts Hrects].
   - auto.
-  - simpl in H; unfold freeVarTerms in H;
-      fold (freeVarTerm L (substT L t v s)) in H;
-      fold (freeVarTerms L n (substTs L n ts v s)) in H.
-    unfold freeVarTerms; fold (freeVarTerm L t); fold (freeVarTerms L n ts).
+  - simpl in H; unfold freeVarTs in H;
+      fold (freeVarT L (substT L t v s)) in H;
+      fold (freeVarTs L n (substTs L n ts v s)) in H.
+    unfold freeVarTs; fold (freeVarT L t); fold (freeVarTs L n ts).
     induction (in_app_or _ _ _ H) as [H1 | H1].
     + apply in_or_app; left; eapply freeVarSubTerm4.
       * apply H1.
       * intro H2; elim H0.
-        unfold freeVarTerms; fold (freeVarTerm L t);
-          fold (freeVarTerms L n ts); apply in_or_app; now left.
+        unfold freeVarTs; fold (freeVarT L t);
+          fold (freeVarTs L n ts); apply in_or_app; now left.
     + apply in_or_app; right; eapply Hrects. 
       * apply H1.
-      * intro H2; elim H0; unfold freeVarTerms;
-          fold (freeVarTerm L t); fold (freeVarTerms L n ts).
+      * intro H2; elim H0; unfold freeVarTs;
+          fold (freeVarT L t); fold (freeVarTs L n ts).
         apply in_or_app; now right.
 Qed.
 
@@ -471,8 +471,8 @@ Proof.
     simpl in H1; rewrite subFormulaForall in H0.
     induction (eq_nat_dec v v0) as [a0 | ?]. 
     + apply H0.
-    + induction (In_dec eq_nat_dec v (freeVarTerm L s)) as [a0 | ?].
-      * set (nv := newVar (v0 :: freeVarTerm L s ++ freeVarF L a)).
+    + induction (In_dec eq_nat_dec v (freeVarT L s)) as [a0 | ?].
+      * set (nv := newVar (v0 :: freeVarT L s ++ freeVarF L a)).
         simpl in H0.
         assert
           (H2: In x
@@ -486,7 +486,7 @@ Proof.
           - apply H2.
           - intros H3; induction (freeVarSubFormula3 _ _ _ _ H3).
             + auto.
-            + elim (newVar1 (v0 :: freeVarTerm L s ++ freeVarF L a)).
+            + elim (newVar1 (v0 :: freeVarT L s ++ freeVarF L a)).
               fold nv; induction H4 as [H4| H4].
               * rewrite H4; simpl; now left.  
               * elim H4.
@@ -506,13 +506,13 @@ Proof.
 Qed.
 
 Lemma subTermNil (t : Term) (v : nat) (s : Term):
- ~ In v (freeVarTerm L t) -> substT L t v s = t.
+ ~ In v (freeVarT L t) -> substT L t v s = t.
 Proof.
   elim t using
     Term_Terms_ind
     with
     (P0 := fun (n : nat) (ts : fol.Terms L n) =>
-             ~ In v (freeVarTerms L n ts) -> substTs L n ts v s = ts).
+             ~ In v (freeVarTs L n ts) -> substTs L n ts v s = ts).
   - intros n H; simpl in H; rewrite subTermVar2.
     + reflexivity.
     + intro H0; apply H; left; auto. 
@@ -520,7 +520,7 @@ Proof.
     + reflexivity.
     + apply H0.
   - reflexivity. 
-  - intros n t0 H t1 H0 H1; simpl; unfold freeVarTerms in H1.
+  - intros n t0 H t1 H0 H1; simpl; unfold freeVarTs in H1.
     rewrite H0.
     + rewrite H.
       * reflexivity.
@@ -529,7 +529,7 @@ Proof.
 Qed.
  
 Lemma subTermTrans  (t : Term) (v1 v2 : nat) (s : Term):
- ~ In v2 (List.remove  eq_nat_dec v1 (freeVarTerm L t)) ->
+ ~ In v2 (List.remove  eq_nat_dec v1 (freeVarT L t)) ->
  substT L (substT L t v1 (var v2)) v2 s =
  substT L t v1 s.
 Proof.
@@ -537,7 +537,7 @@ Proof.
     Term_Terms_ind
     with
     (P0 := fun (n : nat) (ts : fol.Terms L n) =>
-             ~ In v2 (List.remove eq_nat_dec v1 (freeVarTerms L n ts)) ->
+             ~ In v2 (List.remove eq_nat_dec v1 (freeVarTs L n ts)) ->
              substTs L n (substTs L n ts v1 (var v2)) v2 s =
                substTs L n ts v1 s).
   - intros n H; simpl; induction (eq_nat_dec v1 n) as [? | b].
@@ -551,7 +551,7 @@ Proof.
     + reflexivity.
     + apply H0.
   - auto.
-  - intros n t0 H t1 H0 H1; simpl; unfold freeVarTerms in H1.
+  - intros n t0 H t1 H0 H1; simpl; unfold freeVarTs in H1.
     rewrite H0.
     * rewrite H. 
       -- reflexivity.
@@ -566,8 +566,8 @@ Qed.
 
 Lemma subTermExch  (t : Term) (v1 v2 : nat) (s1 s2 : Term):
  v1 <> v2 ->
- ~ In v2 (freeVarTerm L s1) ->
- ~ In v1 (freeVarTerm L s2) ->
+ ~ In v2 (freeVarT L s1) ->
+ ~ In v1 (freeVarT L s2) ->
  substT L (substT L t v1 s1) v2 s2 =
  substT L (substT L t v2 s2) v1 s1.
 Proof.
@@ -576,8 +576,8 @@ Proof.
     with
     (P0 := fun (n : nat) (ts : fol.Terms L n) =>
              v1 <> v2 ->
-             ~ In v2 (freeVarTerm L s1) ->
-             ~ In v1 (freeVarTerm L s2) ->
+             ~ In v2 (freeVarT L s1) ->
+             ~ In v1 (freeVarT L s2) ->
              substTs L n (substTs L n ts v1 s1) v2 s2 =
                substTs L n (substTs L n ts v2 s2) v1 s1).
  - intros n H H0 H1; simpl; induction (eq_nat_dec v1 n) as [a | ?].
@@ -596,11 +596,11 @@ Proof.
 Qed.
 
 Lemma subTermsNil  (n : nat) (ts : Terms n) (v : nat) (s : Term):
- ~ In v (freeVarTerms L n ts) -> substTs L n ts v s = ts.
+ ~ In v (freeVarTs L n ts) -> substTs L n ts v s = ts.
 Proof.
   intros H; induction ts as [| n t ts Hrects].
   - auto.
-  - simpl; unfold freeVarTerms in H; rewrite Hrects.
+  - simpl; unfold freeVarTs in H; rewrite Hrects.
     + rewrite subTermNil.
       * reflexivity.
       * intro H0; elim H; apply in_or_app; auto.
@@ -608,13 +608,13 @@ Proof.
 Qed.
 
 Lemma subTermsTrans (n : nat) (ts : Terms n) (v1 v2 : nat) (s : Term):
- ~ In v2 (List.remove  eq_nat_dec v1 (freeVarTerms L n ts)) ->
+ ~ In v2 (List.remove  eq_nat_dec v1 (freeVarTs L n ts)) ->
  substTs L n (substTs L n ts v1 (var v2)) v2 s =
  substTs L n ts v1 s.
 Proof.
   intros H; induction ts as [| n t ts Hrects].
   - auto.
-  - simpl; unfold freeVarTerms in H; rewrite Hrects.
+  - simpl; unfold freeVarTs in H; rewrite Hrects.
     + rewrite subTermTrans.
       * reflexivity.
       * intro H0; elim H; apply in_in_remove.
@@ -628,8 +628,8 @@ Qed.
 Lemma subTermsExch  (n : nat) (ts : Terms n) (v1 v2 : nat) 
   (s1 s2 : Term):
   v1 <> v2 ->
-  ~ In v2 (freeVarTerm L s1) ->
-  ~ In v1 (freeVarTerm L s2) ->
+  ~ In v2 (freeVarT L s1) ->
+  ~ In v1 (freeVarT L s2) ->
   substTs L n (substTs L n ts v1 s1) v2 s2 =
     substTs L n (substTs L n ts v2 s2) v1 s1.
 Proof.
@@ -666,8 +666,8 @@ Remark subFormulaNTE  (f : Formula):
                (substF L f v1 s))) /\
       (forall (v1 v2 : nat) (s1 s2 : Term),
           v1 <> v2 ->
-          ~ In v2 (freeVarTerm L s1) ->
-          ~ In v1 (freeVarTerm L s2) ->
+          ~ In v2 (freeVarT L s1) ->
+          ~ In v1 (freeVarT L s2) ->
           SysPrf T
             (iffH (substF L (substF L f v1 s1) v2 s2)
                (substF L (substF L f v2 s2) v1 s1))).
@@ -1563,8 +1563,8 @@ Proof.
       assert
         (H3: forall (v1 v2 : nat) (s1 s2 : Term),
             v1 <> v2 ->
-            ~ In v2 (freeVarTerm L s1) ->
-            ~ In v1 (freeVarTerm L s2) ->
+            ~ In v2 (freeVarT L s1) ->
+            ~ In v1 (freeVarT L s2) ->
             SysPrf T
               (impH
                  (substF L (substF L (forallH v a) v1 s1)
@@ -2599,8 +2599,8 @@ Qed.
 Lemma subFormulaExch :
  forall (f : Formula) (T : System) (v1 v2 : nat) (s1 s2 : Term),
  v1 <> v2 ->
- ~ In v2 (freeVarTerm L s1) ->
- ~ In v1 (freeVarTerm L s2) ->
+ ~ In v2 (freeVarT L s1) ->
+ ~ In v1 (freeVarT L s2) ->
  SysPrf T
    (iffH (substF L (substF L f v1 s1) v2 s2)
       (substF L (substF L f v2 s2) v1 s1)).
